Execute AST with big-step semantics

AST.v
@@ -1,7 +1,9 @@
 Require Import Coq.Lists.List. Import ListNotations.
+Require Import Coq.Strings.String.
 Require Import Coq.Strings.Byte.
 Require Import Coq.ZArith.ZArith.
 Require Import BF.Byte.
+Require Import BF.VM.
 Require Import BF.Token.
 
 Inductive ast : Type :=
@@ -13,6 +15,42 @@ Inductive ast : Type :=
   | AInput (a : ast)
   | ALoop (body : ast) (a : ast)
   | AEnd.
+
+Inductive ast_execute : ast -> vm -> vm -> Prop :=
+  | E_ARight_nil : forall next l c o i v'',
+      ast_execute next (VM (c :: l) x00 [] o i) v'' ->
+      ast_execute (ARight next) (VM l c [] o i) v''
+  | E_ARight : forall next l c x r' o i v'',
+      ast_execute next (VM (c :: l) x r' o i) v'' ->
+      ast_execute (ARight next) (VM l c (x :: r') o i) v''
+  | E_ALeft_nil : forall next x l' o i v'',
+      ast_execute next (VM l' x [] o i) v'' ->
+      ast_execute (ALeft next) (VM (x :: l') x00 [] o i) v''
+  | E_ALeft : forall next x l' c r o i v'',
+      ast_execute next (VM l' x (c :: r) o i) v'' ->
+      ast_execute (ALeft next) (VM (x :: l') c r o i) v''
+  | E_AInc : forall next l c r o i v'',
+      ast_execute next (VM l (byte_add x01 c) r o i) v'' ->
+      ast_execute (AInc next) (VM l c r o i) v''
+  | E_ADec : forall next l c r o i v'',
+      ast_execute next (VM l (byte_add xff c) r o i) v'' ->
+      ast_execute (ADec next) (VM l c r o i) v''
+  | E_AOutput : forall next l c r o i v'',
+      ast_execute next (VM l c r (c :: o) i) v'' ->
+      ast_execute (AOutput next) (VM l c r o i) v''
+  | E_AInput : forall next l c r o x i' v'',
+      ast_execute next (VM l x r o i') v'' ->
+      ast_execute (AInput next) (VM l c r o (x :: i')) v''
+  | E_ALoop_0 : forall body next l r o i v',
+      ast_execute next (VM l x00 r o i) v' ->
+      ast_execute (ALoop body next) (VM l x00 r o i) v'
+  | E_ALoop : forall body next l c r o i v' v'',
+      c <> x00 ->
+      ast_execute body (VM l c r o i) v' ->
+      ast_execute (ALoop body next) v' v'' ->
+      ast_execute (ALoop body next) (VM l c r o i) v''
+  | E_AEnd : forall v,
+      ast_execute AEnd v v.
 
 Fixpoint parse' (ts : list token) : ast * list ast :=
   match ts with
@@ -52,22 +90,24 @@ Fixpoint flatten (a : ast) : list token :=
   | AEnd => []
   end.
 
-Fixpoint ast_cons_repeat (node : ast -> ast) (n : nat) (a : ast) : ast :=
-  match n with
-  | O => a
-  | S n' => node (ast_cons_repeat node n' a)
-  end.
-
 Definition ast_cons_move (n : Z) (a : ast) : ast :=
   match n with
   | Z0 => a
-  | Zpos p => ast_cons_repeat ARight (Pos.to_nat p) a
-  | Zneg p => ast_cons_repeat ALeft (Pos.to_nat p) a
+  | Zpos p => repeat_apply ARight (Pos.to_nat p) a
+  | Zneg p => repeat_apply ALeft (Pos.to_nat p) a
   end.
 
 Definition ast_cons_add (n : byte) (a : ast) : ast :=
   match byte_to_Z n with
   | Z0 => a
-  | Zpos p => ast_cons_repeat AInc (Pos.to_nat p) a
-  | Zneg p => ast_cons_repeat ADec (Pos.to_nat p) a
+  | Zpos p => repeat_apply AInc (Pos.to_nat p) a
+  | Zneg p => repeat_apply ADec (Pos.to_nat p) a
   end.
+
+Example test_ast_execute : forall a,
+  parse (lex "++>+++[-<++>]<-.") = Some a ->
+  ast_execute a (vm_make []) (VM [] x07 [] [x07] []).
+Proof.
+  intros. inversion H; subst; clear H.
+  repeat (constructor || (eapply E_ALoop; [discriminate | |])).
+Qed.
