VM.v
@@ -1,0 +1,61 @@
+Require Import Coq.Lists.List. Import ListNotations.
+Require Import Coq.Strings.Byte.
+Require Import Coq.ZArith.ZArith.
+Import IfNotations.
+Require Import BF.Byte.
+
+Fixpoint repeat_apply {A : Type} (f : A -> A) (n : nat) (a : A) : A :=
+  match n with
+  | O => a
+  | S n' => f (repeat_apply f n' a)
+  end.
+
+Fixpoint repeat_apply_option {A : Type} (f : A -> option A) (n : nat) (a : A) : option A :=
+  match n with
+  | O => Some a
+  | S n' => if repeat_apply_option f n' a is Some a' then f a' else None
+  end.
+
+Inductive vm : Type :=
+  VM (l : list byte) (* cells to the left *)
+     (c : byte) (* current cell *)
+     (r : list byte) (* cells to the right *)
+     (o : list byte) (* outputs *)
+     (i : list byte). (* inputs *)
+
+Definition vm_make (i : list byte) : vm := VM [] x00 [] [] i.
+
+Definition vm_get_cell (v : vm) : byte :=
+  match v with VM _ c _ _ _ => c end.
+
+Definition vm_move_left (v : vm) : option vm :=
+  match v with
+  | VM (l :: l') x00 [] o i => Some (VM l' l [] o i)
+  | VM (l :: l') c r o i => Some (VM l' l (c :: r) o i)
+  | _ => None
+  end.
+
+Definition vm_move_right (v : vm) : vm :=
+  match v with
+  | VM l c (r :: r') o i => VM (c :: l) r r' o i
+  | VM l c [] o i => VM (c :: l) x00 [] o i
+  end.
+
+Definition vm_move (n : Z) (v : vm) : option vm :=
+  match n with
+  | Z0 => Some v
+  | Zpos p => Some (repeat_apply vm_move_right (Pos.to_nat p) v)
+  | Zneg p => repeat_apply_option vm_move_left (Pos.to_nat p) v
+  end.
+
+Definition vm_add (n : byte) (v : vm) : vm :=
+  match v with VM l c r o i => VM l (byte_add n c) r o i end.
+
+Definition vm_output (v : vm) : vm :=
+  match v with VM l c r o i => VM l c r (c :: o) i end.
+
+Definition vm_input (v : vm) : option vm :=
+  match v with
+  | VM l _ r o (c :: i') => Some (VM l c r o i')
+  | _ => None
+  end.
